XDOC now has a new, "fancy" viewer.
   Preview: http://fv.centtech.com/fancy/    (slow loading, see below)
     (Note: will be taken down soon)

The basic idea is that instead of generating everything (index and content
pages) ahead of time as thousands of individual .xml and .xdoc-link files, I
just preprocess everything and then write out the XDOC database as JSON
formatted data.

On the ACL2 side, this approach simplifies the XDOC lisp code by a good deal
(well---or at least, it *could* simplify the code, if I got rid of the old
"save" command, but I've left that in for now).  It also speeds up creating
manuals by a good bit (it cuts about a minute off of centaur/doc.lisp; with the
actual save command is down to about 25 seconds.)

On the display side, things are more complex but much fancier.  The JSON
version of the documentation database can be easily loaded into JavaScript, so
the entire display can be handled with ordinary web programming.  The new
viewer has a much richer navigation system with both hierarchical and flat
organizations, A-Z buttons for the flat navigation, a "jump to topic" box with
typeahead support, etc.  It also has a much fancier content display that lets
you expand subtopics, etc.  This is really cool: try it for instance on

       http://fv.centtech.com/fancy/?topic=ACL2____RULESETS

Deployment is somewhat easier than before.  There are far fewer files and no
need to install Xalan or run "make" any more.

One problem is size.  The encoded database is large (around 20 MB), and we just
load the whole stupid thing in.  This is just fine (great, even) when reading
from local storage or from an intranet site on a LAN.  But it's definitely not
a good solution for public facing web sites like the fv.centtech.com above, and
external users will probably see a considerable delay while the page boots up.

For a public-facing web site, it should be quite easy to stuff the big xdata.js
part of the database into, say, an sqlite3 database and grab the long strings
on demand via AJAX queries.  I'll probably add this soon to make a much faster
version of the fancy web site.

books/xdoc/fancy/xdoc.js
@@ -1,0 +1,760 @@
+/*
+; XDOC Documentation System for ACL2
+; Copyright (C) 2009-2013 Centaur Technology
+;
+; Contact:
+;   Centaur Technology Formal Verification Group
+;   7600-C N. Capital of Texas Highway, Suite 300, Austin, TX 78731, USA.
+;   http://www.centtech.com/
+;
+; This program is free software; you can redistribute it and/or modify it under
+; the terms of the GNU General Public License as published by the Free Software
+; Foundation; either version 2 of the License, or (at your option) any later
+; version.  This program is distributed in the hope that it will be useful but
+; WITHOUT ANY WARRANTY; without even the implied warranty of MERCHANTABILITY or
+; FITNESS FOR A PARTICULAR PURPOSE.  See the GNU General Public License for
+; more details.  You should have received a copy of the GNU General Public
+; License along with this program; if not, write to the Free Software
+; Foundation, Inc., 51 Franklin Street, Suite 500, Boston, MA 02110-1335, USA.
+;
+; Original author: Jared Davis <jared@centtech.com>
+*/
+
+var TOP_KEY = "ACL2____TOP";
+var xindex_loaded = false;
+var xdata_loaded = false;
+
+
+
+// --------------------------------------------------------------------------
+//
+//                         RANDOM UTILITIES
+//
+// --------------------------------------------------------------------------
+
+// Initialize an XSLT processor for XDOC --> HTML conversion
+var xslt_processor = new XSLTProcessor();
+{
+    var xslt_plain = $.base64.decode(xslt_base64);
+    var xslt_dom = $.parseXML(xslt_plain);
+    xslt_processor.importStylesheet(xslt_dom);
+}
+
+function wrap_xdoc_fragment(str) {
+    var wrap = "<!DOCTYPE xdoc [";
+    wrap += "<!ENTITY mdash \"&#8212;\">";
+    wrap += "<!ENTITY rarr \"&#8594;\">";
+    wrap += "<!ENTITY nbsp \"&#160;\">";
+    wrap += "]>";
+    wrap += "<root>" + str + "</root>";
+    return wrap;
+}
+
+function render_text (str) { // XDOC Markup (string) --> Plain Text Fragment
+    var xml = $.parseXML(wrap_xdoc_fragment(str));
+    var dom = xslt_processor.transformToFragment(xml,document);
+    var str = $(dom).text();
+
+    // It's not clear to me whether this is good or bad.  The basic problem
+    // is that strings like "short" strings might legitimately have quotes
+    // or apostrophes in them.  This is no problem if we're going to stick the
+    // render_text into a paragraph or something like that.  But it *is* a
+    // problem if we're going to stick it into an attribute like a tooltip
+    // or similar.  So, just to avoid problems like that, make sure the resulting
+    // string is free of " and ' characters.
+    return String(str)
+             .replace(/"/g, '&quot;')
+	     .replace(/'/g, '&apos;');
+}
+
+function render_html (str) { // XDOC Markup (string) --> HTML DOM Fragment
+    var xml = $.parseXML(wrap_xdoc_fragment(str));
+    var dom = xslt_processor.transformToFragment(xml,document);
+    return dom;
+}
+
+function alphanum(a, b) { // Alphanumeric comparison (for nice sorting)
+  // Credit: http://my.opera.com/GreyWyvern/blog/show.dml/1671288
+  function chunkify(t) {
+    var tz = [], x = 0, y = -1, n = 0, i, j;
+
+    while ((i = (j = t.charAt(x++)).charCodeAt(0))) {
+      var m = (i == 46 || (i >=48 && i <= 57));
+      if (m !== n) {
+        tz[++y] = "";
+        n = m;
+      }
+      tz[y] += j;
+    }
+    return tz;
+  }
+
+  var aa = chunkify(a);
+  var bb = chunkify(b);
+
+  for (var x = 0; aa[x] && bb[x]; x++) {
+    if (aa[x] !== bb[x]) {
+      var c = Number(aa[x]), d = Number(bb[x]);
+      if (c == aa[x] && d == bb[x]) {
+        return c - d;
+      } else return (aa[x] > bb[x]) ? 1 : -1;
+    }
+  }
+  return aa.length - bb.length;
+}
+
+function starts_with_alpha(str) {
+    var little_a = "a".charCodeAt(0);
+    var little_z = "z".charCodeAt(0);
+    var big_a = "A".charCodeAt(0);
+    var big_z = "Z".charCodeAt(0);
+    var code = str.charCodeAt(0);
+    return (little_a <= code && code <= little_z)
+        || (   big_a <= code && code <= big_z   );
+}
+
+var waitmsg = 0;
+function please_wait() {
+    var msgs = ["Still loading",
+	        "Gah, what's taking so long?",
+		"Man, tubes must be clogged...",
+		"The boy has no patience.",
+		"It's not ready yet!",
+  	        "Dude, stop clicking already!"];
+    $("#still_loading").html("<p>" + msgs[waitmsg] + "</p>");
+    $("#still_loading").fadeIn(100).delay(500).fadeOut(100);
+    waitmsg = waitmsg + 1;
+    if (waitmsg == msgs.length)
+	waitmsg = msgs.length - 1;
+}
+
+
+// --------------------------------------------------------------------------
+//
+//                          MAIN DATA STRUCTURES
+//
+// --------------------------------------------------------------------------
+//
+// The XDOC database is split up into two files: XINDEX and XDATA.  Both of
+// these files are generated ahead of time by the ACL2 code for XDOC.
+//    - xindex is smaller and contains just the navigation data
+//    - xdata is larger and has the full "long" strings for each topic
+//
+// We load these files lazily to make the page seem to appear faster!  This
+// means you have to sort of be aware of when the data becomes available.  We
+// load xindex first, then once it's complete we load xdata.
+//
+// XINDEX is smaller.  In the xindex.js file, you can roughly think of XINDEX
+// as being a mapping from:
+//
+//    xindex:   KEY -> { "name":"xml encoded nice topic name",
+//                       "pkeys":[array of KEY for parents],
+//                       "short":"xml encoded short topic description",
+//                       "rawname":"non-encoded symbol-name (no package)" }
+//
+// Except that actually we use an array instead of a hash (which saves about
+// 400 KB) from centaur/doc.lisp at the time of this writing.  The indexes
+// into the array are as follows.  These MUST AGREE WITH SAVE-FANCY.LISP:
+
+var XI_NAME    = 0;
+var XI_RAWNAME = 1;
+var XI_PKEYS   = 2;
+var XI_SHORT   = 3;
+
+// But once XINDEX gets loaded, we also fill in some additional information.
+// In particular, it is useful to have a list of all of a topic's children.
+// (This is fast and easy to construct, given that xindex already maps each
+// child to its parents).  So we fill in each XINDEX entry with a "children"
+// field.
+
+var XI_CHILDREN = 4; // array of keys for children
+
+
+// The XDATA table is simpler:
+//
+//   xdata:         KEY -> {"pnames" : [array of xml encoded nice parent names],
+//                          "long"   : "xml encoded long topic description"}
+//
+// Except that again we use an array to save a tiny amount of space.
+
+var XD_PNAMES = 0;
+var XD_LONG = 1;
+
+
+
+
+function xindex_add_children() { // assumes xindex is populated
+    for(var child_key in xindex) {
+	var parent_keys = xindex[child_key][XI_PKEYS];
+	for(var i in parent_keys) {
+	    var parent_key = parent_keys[i];
+	    // It's incorrect, but possible for a child topic to list parents
+	    // that don't exist, so we have to make sure it really exists:
+	    if (parent_key in xindex) {
+		var parent_node = xindex[parent_key];
+		if (!parent_node[XI_CHILDREN])
+		    parent_node[XI_CHILDREN] = [];
+		parent_node[XI_CHILDREN].push(child_key);
+	    }
+	}
+    }
+    xindex_loaded = true;
+}
+
+function key_title(key)
+{
+    return (key in xindex)
+	     ? ("XDOC &mdash; " + xindex[key][XI_NAME])
+	     : ("XDOC &mdash; " + key);
+}
+
+function key_sorted_children(key) { // Returns a nicely sorted array of child_keys
+    if (!(key in xindex)) {
+	return [];
+    }
+    var info = xindex[key];
+    var children = info[XI_CHILDREN];
+
+    var tmp = [];
+    for(i in children) {
+	var child_key = children[i];
+	var rawname = xindex[child_key][XI_RAWNAME];
+	tmp.push({key:child_key, rawname:rawname});
+    }
+    tmp.sort(function(a,b) { return alphanum(a.rawname, b.rawname); });
+
+    var ret = [];
+    for(i in tmp) {
+	ret.push(tmp[i].key);
+    }
+    return ret;
+}
+
+
+
+// --------------------------------------------------------------------------
+//
+//                          NAVIGATION TREE
+//
+// --------------------------------------------------------------------------
+//
+// Turning the index into a navigation tree is made more complicated by the
+// following mismatch.
+//
+//    In the xindex, each topic can have many parents.
+//    In the navigation window we show a tree, i.e., there's just one parent!
+//
+// To reconcile this difference, we basically "replicate" topics in the tree.
+// For instance, we could show the user something like this:
+//
+//     TOP
+//      - Parent1
+//          OurTopic  -------+   (occurrence 1)
+//            Child1         |
+//            Child2         |   The topic and its children are "replicated"
+//      - Parent2            |
+//          OurTopic  -------+   (occurrence 2)
+//            Child1
+//            Child2
+//
+// The tricky part is: what happens when the user clicks on Occurrence 1 of
+// OurTopic?  In this case, we want to:
+//
+//     - hide/show the children only underneath occurrence 1, but
+//     - NOT change the state of occurrence 2 or its children!
+//
+// This means that we need to be able to distinguish between OCCURRENCES of
+// topics, not just the topic names/keys themselves.
+//
+// To do this, we are going to dumbly assign a "unique identifiers" to each
+// node in the navigation window.
+//
+// To simplify some things, we insist that the TOP topic gets identifier 0.
+// But otherwise, there's no reason we even need to assign these indices until
+// we can see the node.  So we lazily assign IDs to other nodes, as they become
+// visible in the navigation window.  These assignments are stored in the ID
+// table:
+
+var nav_id_table = []; // map of ID to {"key":KEY,"ever_expanded":bool}
+
+function nav_make_node(key) {
+    // Create the navigation entry for a new occurrence of KEY.
+    var id = nav_id_table.length;
+    nav_id_table[id] = {"key":key, "ever_expanded":false};
+
+    var info = xindex[key];
+    var name = info[XI_NAME];
+    var tooltip = "<p>" + render_text(info[XI_SHORT]) + "</p>";
+
+    var node = "<ul class=\"hindex\" id=\"_nav" + id + "\">";
+    node += "<li><nobr>";
+    if (!info[XI_CHILDREN]) {
+	node += "<img src=\"leaf.png\"/>";
+    }
+    else {
+	node += "<a id=\"_nav_ilink" + id + "\" ";
+	node += " href=\"javascript:nav_expand(" + id + ")\">";
+	node += "<img src=\"plus.png\" id=\"_nav_img" + id + "\"/>";
+	node += "</a>";
+    }
+    node += "<a id=\"_golink" + id + "\" href=\"javascript:nav_go(" + id
+	    + ")\" data-powertip=\"" + tooltip + "\">";
+    node += name;
+    node += "</a>";
+    node += "</nobr>";
+    node += "<li><ul class=\"hindex\" id=\"_nav_tree" + id + "\"></ul></li>";
+    return node;
+}
+
+function nav_activate_tooltip(id) {
+    // This sort of "should" be part of nav_make_node, but it can't be because
+    // the node has to be properly installed into the document before jquery
+    // can find it.
+    $("#_golink" + id).powerTip({placement:'se',smartPlacement: true});
+}
+
+function nav_expand(id) {
+    // The user has just clicked on a node.  We may or may not have expanded it
+    // already.  If we haven't expanded it before, we need to make nodes for
+    // its children and add them.  If we have expanded it already, then we must
+    // have subsequently collapsed it, and we just want to make it visible
+    // again.
+    $("#_nav_img" + id).attr("src", "minus.png");
+    $("#_nav_ilink" + id).attr("href", "javascript:nav_retract(" + id + ")");
+    var key = nav_id_table[id]["key"];
+
+    if(nav_id_table[id]["ever_expanded"]) {
+	$("#_nav_tree" + id).show();
+	return;
+    }
+
+    nav_id_table[id]["ever_expanded"] = true;
+    var info = xindex[key];
+    var children = key_sorted_children(key);
+
+    var start = nav_id_table.length; // stupid hack for tooltip activation
+    var exp = "";
+    for(i in children) {
+	exp += nav_make_node(children[i]);
+    }
+    $("#_nav_tree" + id).append(exp);
+
+    // Activate only the tooltips that we have just added.  (If we try to
+    // activate them more than once, they don't seem to work.)
+    for(var i = start; i < nav_id_table.length; ++i) {
+	nav_activate_tooltip(i);
+    }
+}
+
+function nav_retract(id)
+{
+    $("#_nav_img" + id).attr("src", "plus.png");
+    $("#_nav_ilink" + id).attr("href", "JavaScript:nav_expand(" + id + ")");
+    $("#_nav_tree" + id).hide();
+}
+
+var nav_mode = "tree";
+var nav_tree_top = 0;
+var nav_flat_top = 0;
+var nav_flat_ever_shown = false;
+
+function nav_tree() {
+    if (!xindex_loaded) {
+	please_wait();
+	return;
+    }
+    if (nav_mode == "tree") { return; }
+    nav_flat_top = $("#left").scrollTop();
+    $("#left").scrollTop(nav_tree_top);
+    $("#flat").hide();
+    $("#nav").show();
+    nav_mode = "tree";
+}
+
+function nav_flat() {
+    if (!xindex_loaded) {
+	please_wait();
+	return;
+    }
+    if (nav_mode == "flat") { return; }
+    nav_tree_top = $("#left").scrollTop();
+    $("#left").scrollTop(nav_flat_top);
+    $("#nav").hide();
+    $("#flat").show();
+    nav_mode = "flat";
+
+    if (nav_flat_ever_shown) {
+       // Nothing to do, we've already built the flat index.
+       return;
+    }
+
+    $("#flat").html("");
+
+    nav_flat_ever_shown = true;
+
+    var myarr = [];
+    for(key in xindex) {
+	myarr.push({key:key, rawname: xindex[key][XI_RAWNAME]});
+    }
+    myarr.sort(function(a,b) { return alphanum(a.rawname, b.rawname); });
+
+    var dl = jQuery("<ul></ul>");
+    var current_startchar = "";
+    for(i in myarr) {
+	var key = myarr[i].key;
+	var info = xindex[key];
+	var name = info[XI_NAME];
+	var rawname = info[XI_RAWNAME];
+	var tooltip = "<p>" + render_text(info[XI_SHORT]) + "</p>";
+	if ((rawname.charAt(0) != current_startchar) && starts_with_alpha(rawname)) {
+	    current_startchar = rawname.charAt(0).toUpperCase();
+	    dl.append("<li class=\"flatsec\" id=\"flat_startchar_" + current_startchar + "\"><b>"
+		      + current_startchar + "</b></li>");
+	}
+
+	dl.append("<li><a class=\"flatnav\""
+		  + " href=\"JavaScript:action_go_key('" + key + "')\""
+		  + " data-powertip=\"" + tooltip + "\">"
+		  + name
+		  + "</li>");
+    }
+    $("#flat").append(dl);
+    $(".flatnav").powerTip({placement:'se',smartPlacement: true});
+}
+
+function nav_flat_tochar(c) {
+    nav_flat();
+    $("#left").scrollTop(0);
+    var target = $("#flat_startchar_" + c).offset().top;
+    var adjust = target - $("#left").offset().top;
+    $("#left").scrollTop(adjust);
+}
+
+function nav_go(id)
+{
+    var key = nav_id_table[id]["key"];
+    action_go_key(key);
+}
+
+
+
+// --------------------------------------------------------------------------
+//
+//                          MAIN DATA DISPLAY
+//
+// --------------------------------------------------------------------------
+//
+// My first cut at the data display didn't have any way to expand subtopics,
+// and that was nice and simple.  But subtopic expansion seems like a cool
+// feature.  To support it recursively, we run into the same multi-parent
+// problem as above in the hierarchical navigation tree.  The same solution
+// works again.  But this time we need to clear the ID table every time we
+// go to a new topic.
+
+var dat_id_table = []; // map of Occurrence ID to {"key":KEY,"ever_expanded":bool}
+
+function dat_load_parents(key) {
+    var info = xindex[key];
+    var parent_keys = info[XI_PKEYS];
+    var parent_names = xdata[key][XD_PNAMES];
+    var acc = "";
+    if (parent_keys.length == 0) {
+	$("#parents").hide();
+	$("#parents").html("");
+	return;
+    }
+    acc += "<ul>";
+    for(var i in parent_keys) {
+	var pkey = parent_keys[i];
+	var pname = parent_names[i];
+	var tooltip = "Error: parent topic is missing!";
+	if (pkey in xindex) {
+	    var pinfo = xindex[pkey];
+	    tooltip = render_text(pinfo[XI_SHORT]);
+	}
+	acc += "<li>";
+	acc += "<a href=\"javascript:action_go_key('" + pkey + "')\""
+	    + "data-powertip=\"<p>" + tooltip + "</p>\">";
+	acc += pname;
+	acc += "</a>";
+	acc += "</li>\n";
+    }
+    acc += "</ul>";
+    $("#parents").html(acc);
+    $("#parents a").powerTip({placement:'se',smartPlacement: true});
+    $("#parents").show();
+}
+
+function dat_short_subtopics(key)
+{
+    var info = xindex[key];
+    var children = key_sorted_children(key);
+
+    var dl = jQuery("<div></div>");
+    for(var i in children) {
+	var child_key = children[i];
+	var child_info = xindex[child_key];
+	dl.append("<dt><a href=\"javascript:action_go_key('" + child_key + "')\">"
+		  + child_info[XI_NAME]
+		  + "</dt>");
+	var dd = jQuery("<dd></dd>");
+	dd.append(render_html(child_info[XI_SHORT]));
+	dl.append(dd);
+    }
+    return dl;
+}
+
+function dat_expand(dat_id)
+{
+    $("#_dat_img" + dat_id).attr("src", "collapse_subtopics.png");
+    $("#_dat_ilink" + dat_id).attr("href", "JavaScript:dat_collapse(" + dat_id + ")");
+    $("#_dat_short" + dat_id).hide();
+    $("#_dat_long" + dat_id).show();
+
+    if (dat_id_table[dat_id]["ever_expanded"] == true) {
+	// Already showed it, nothing more to do
+	return;
+    }
+
+    dat_id_table[dat_id]["ever_expanded"] = true;
+    var key = dat_id_table[dat_id]["key"];
+    var info = xindex[key];
+    var children = key_sorted_children(key);
+
+    var div = $("#_dat_long" + dat_id);
+    for(i in children) {
+	var child_key = children[i];
+	div.append(dat_long_topic(child_key));
+	if (i != children.length - 1) {
+	    div.append("<hr></hr>");
+	}
+    }
+}
+
+function dat_collapse(dat_id)
+{
+    $("#_dat_img" + dat_id).attr("src", "expand_subtopics.png");
+    $("#_dat_ilink" + dat_id).attr("href", "JavaScript:dat_expand(" + dat_id + ")");
+    $("#_dat_short" + dat_id).show();
+    $("#_dat_long" + dat_id).hide();
+}
+
+function dat_long_topic(key)
+{
+    var dat_id = dat_id_table.length;
+    dat_id_table[dat_id] = {"key":key, "ever_expanded":false};
+
+    var div = jQuery("<div></div>");
+    if (!(key in xindex)) {
+	div.append("<h3>Error: " + key + " not found</h3>");
+	return div;
+    }
+
+    var info = xindex[key];
+    div.append("<h1>" + info[XI_NAME] + "</h1>");
+    var shortp = jQuery("<p></p>");
+    shortp.append(render_html(info[XI_SHORT]));
+    div.append(shortp);
+    div.append(render_html(xdata[key][XD_LONG]));
+    if (info[XI_CHILDREN]) {
+	var acc = "<h3>";
+	acc += "Subtopics ";
+	acc += "<a id=\"_dat_ilink" + dat_id + "\""
+		+ " href=\"javascript:dat_expand(" + dat_id + ")\">";
+	acc += "<img id=\"_dat_img" + dat_id + "\""
+		+ " src=\"expand_subtopics.png\" align=\"top\"/>";
+	acc += "</a>";
+	acc += "</h3>";
+	var sub = jQuery("<dl id=\"_dat_short" + dat_id + "\"></dl>");
+	sub.append(dat_short_subtopics(key));
+	div.append(acc);
+	div.append(sub);
+	div.append("<div id=\"_dat_long" + dat_id + "\" "
+		   + "style=\"display:none\" class=\"dat_long\"></dl>");
+    }
+
+    return div;
+}
+
+function dat_load_key(key)
+{
+    // BOZO consider doing something to find the key in the navigation
+    // hierarchy somewhere, to make the navigation follow along with you?
+
+    $("#parents").html("");
+    $("#data").html("");
+    $("#right").scrollTop(0);
+    dat_id_table = [];
+    dat_load_parents(key);
+    $("#data").append(dat_long_topic(key));
+    $("title").html(key_title(key));
+}
+
+
+
+
+
+
+
+
+// --------------------------------------------------------------------------
+//
+//                    DATA LOADING / INITIALIZATION
+//
+// --------------------------------------------------------------------------
+
+$(document).ready(function()
+{
+    LazyLoad.js('xindex.js', onIndexLoaded);
+    $(".toolbutton").powerTip({placement:'se'});
+});
+
+
+function jump_init() {
+
+    var ta_data = [];
+    for(var key in xindex) {
+	var info = xindex[key];
+	var tokens = [];
+	tokens.push(info[XI_RAWNAME]);
+	var entry = {"value": key,
+		     "nicename": info[XI_NAME],
+		     "short": render_text(info[XI_SHORT]),
+		     "tokens": tokens};
+	ta_data.push(entry);
+    }
+
+    $("#jump").typeahead([{
+	    name: "topics",
+	    local: ta_data,
+	    limit: 6,
+	    template: "<p><b class=\"sf\">{{{nicename}}}</b> &mdash; {{{short}}}<br/>"
+  		     + "<tt>{{value}}</tt></p>",
+	    engine: Hogan
+    }]);
+
+    $("#jump").bind('typeahead:selected', jump_go);
+    $("#jump").bind('typeahead:autocompleted', jump_go);
+    $("#jumpmsg").powerTip({placement:'se'});
+    $("#jump").attr("placeholder", "append");
+    $("#jump").removeAttr("disabled");
+}
+
+function jump_go(obj,datum) {
+    var key = datum["value"];
+    if (key in xindex)
+	action_go_key(key);
+    else
+	alert("Invalid key " + key);
+    $("#jump").val("");
+    $("#jump").typeahead('setQuery', '');
+}
+
+
+function onIndexLoaded()
+{
+    xindex_add_children();
+
+    // Load xdata.js after xindex_add_children because that way we know the
+    // index is fully initialized by the time we run onDataLoaded.
+    LazyLoad.js('xdata.js', onDataLoaded);
+
+    var acc = "";
+    var chars = "ABCDEFGHIJKLMNOPQRSTUVWXYZ";
+    for(i in chars) {
+	var c = chars.charAt(i);
+	acc += "<a href=\"javascript:nav_flat_tochar('" + c + "')\">" + c + "</a>";
+	if (c == "M")
+	    acc += "<br/>";
+    }
+    $("#letters").html(acc);
+
+    var top_node = nav_make_node(TOP_KEY);
+    $("#nav").html(top_node);
+    nav_expand(0);
+    nav_activate_tooltip(0);
+
+    jump_init();
+}
+
+function onDataLoaded()
+{
+    xdata_loaded = true;
+    var params = getPageParameters();
+    var key = params["topic"] || TOP_KEY;
+
+    window.history.replaceState({"key":key}, key_title(key), "?topic=" + key);
+    dat_load_key(key);
+
+    window.addEventListener('popstate',
+			    function(event) {
+				action_go_back(event.state);
+			    });
+}
+
+function getPageParameters ()
+{
+   var ret = {};
+   if (!window.location.toString().match(/\?(.+)$/)) {
+       return ret;
+   }
+   var param_strs = RegExp.$1.split("&");
+   var param_arr = {};
+   for(i in param_strs)
+   {
+      var tmp = param_strs[i].split("=");
+      var key = decodeURI(tmp[0]);
+      var val = decodeURI(tmp[1]);
+      param_arr[key] = val;
+   }
+   return param_arr;
+}
+
+
+function srclink(key)
+{
+    // BOZO stupid hack, eventually generate this without the .xdoc-link part.
+    key = key.replace(".xdoc-link", "");
+    var rawname = key;
+    if (key in xindex) {
+	rawname = xindex[key][XI_RAWNAME];
+    }
+
+    // Fancy Data URL generator
+    var srclink_header =
+	"; -*- mode: xdoc-link -*-\n" +
+	"; This is an XDOC Link file.\n" +
+	"; Ordinarily, you should not see this file.\n" +
+	";\n" +
+	"; If you are viewing this file in a web browser, you probably\n" +
+	"; have not configured your web browser to send .xdoc-link files\n" +
+	"; to Emacs.\n" +
+	";\n" +
+	"; If you are viewing this file in Emacs, you probably have not\n" +
+	"; loaded xdoc.el from the xdoc/ directory.\n" +
+	";\n" +
+	"; For more information, please see \"Emacs Links\" in the XDOC\n" +
+	"; manual.\n\n"
+
+    window.open('data:application/x-acl2-xdoc-link;charset=utf-8,' +
+    encodeURIComponent(srclink_header + rawname));
+}
+
+function action_go_key(key)
+{
+    if (!xdata_loaded) {
+	please_wait();
+	return;
+    }
+    window.history.pushState({"key":key}, key_title(key), "?topic=" + key);
+    dat_load_key(key);
+}
+
+function action_go_back(data) {
+    var key = ("key" in data) ? data["key"] : null;
+    if (key) {
+	dat_load_key(key);
+    }
+}
+
+
