books/str/package.lsp
@@ -27,7 +27,8 @@
              '(quit exit simpler-take list-fix list-equiv rev
                     prefixp str b* assert! repeat
                     listpos sublistp implode explode
-                    a b c d e f g h i j k l m n o p q r s t u v w x y z)
+                    a b c d e f g h i j k l m n o p q r s t u v w x y z
+                    top)
              '(defxdoc defsection lnfix definlined definline
                 define defaggregate unsigned-byte-p signed-byte-p))
 
